Change from func to list as context

common.v
@@ -1,25 +1,48 @@
 From WR Require Import syntax typing.
 From Coq Require Import ssreflect.
 Require Import Psatz.
+From Hammer Require Import Tactics.
 
-Definition good_renaming ξ n Γ m Δ :=
-  (forall i, i < n -> ξ i < m /\ ren_tm ξ (dep_ith Γ i) = dep_ith Δ (ξ i)).
+Definition good_renaming ξ Γ Δ :=
+  forall i A, dep_ith Γ i = Some A ->
+          dep_ith Δ (ξ i) = Some (ren_tm ξ A).
 
-Lemma good_renaming_truncate n m Γ :
-  good_renaming (Nat.add n) m (Nat.add n >> Γ) (n + m) Γ .
-Proof.
-  rewrite /good_renaming.
-  split.
-  - lia.
-  - asimpldep.
-    f_equal. fext => *; asimpl; lia.
+
+Lemma nth_error_skipn {T : Type} n i Γ (A : T) :
+  nth_error (skipn n Γ) i = Some A ->
+  nth_error Γ (n + i) = Some A.
+  move : n i A.
+  elim : Γ.
+  - hauto lq:on rew:off inv:nat ctrs:option.
+  - hauto lq:on rew:off inv:nat ctrs:option.
 Qed.
 
-Lemma good_renaming_truncate' n m Γ :
-  n <= m ->
-  good_renaming (Nat.add n) (m - n) (Nat.add n >> Γ) m Γ.
+Lemma good_renaming_truncate n Γ :
+  good_renaming (Nat.add n) (skipn n Γ) Γ .
 Proof.
-  move => h.
-  replace m with (n + (m - n)) at 2; last by lia.
-  apply good_renaming_truncate.
+  rewrite /good_renaming => i A h.
+  rewrite dep_ith_shift_n in h.
+  remember (nth_error (skipn n Γ) i) as A0 eqn:eq.
+  case : A0 eq h => // A0 eq h.
+  apply eq_sym in eq.
+  apply nth_error_skipn in eq.
+  simpl in h.
+  case : h => * /=; subst.
+  rewrite dep_ith_shift_n.
+  rewrite eq => /=.
+  asimpl.
+  f_equal.
+  f_equal.
+  simpl.
+  rewrite /funcomp.
+  fext. lia.
 Qed.
+
+(* Lemma good_renaming_truncate' n m Γ : *)
+(*   n <= m -> *)
+(*   good_renaming (Nat.add n) (m - n) (Nat.add n >> Γ) m Γ. *)
+(* Proof. *)
+(*   move => h. *)
+(*   replace m with (n + (m - n)) at 2; last by lia. *)
+(*   apply good_renaming_truncate. *)
+(* Qed. *)
